Lean4Lean/Theory.lean
@@ -1,4 +1,3 @@
 import Lean4Lean.Theory.Typing.EnvLemmas
 import Lean4Lean.Theory.Typing.Strong
-import Lean4Lean.Theory.Typing.ParallelReduction
 import Lean4Lean.Theory.Typing.UniqueTyping
